src/coq/ImpCorrectness.v
@@ -21,6 +21,9 @@ Require Import Vellvm.Classes.
 Require Import Vellvm.Imp Vellvm.Maps Vellvm.ImpCEvalFun.
 Import ListNotations.
 Open Scope list_scope.
+Require Import Program.
+
+
 
 (* Move to Compiler.v *)
 Ltac unfold_llvm H :=
@@ -31,23 +34,23 @@ Arguments Z.add _ _ : simpl nomatch.
 
 (* relational specification of aeval ---------------------------------------- *)
 
-Inductive aevalR : Imp.state -> aexp -> nat -> Prop :=
-  | E_ANum  : forall s (ans: nat),
+Inductive aevalR : Imp.state -> aexp -> int64 -> Prop :=
+  | E_ANum  : forall s (ans: int64),
       aevalR s (ANum ans) ans
   | E_AId : forall s id,
       aevalR s (AId id) (s id)
-  | E_APlus : forall s (a1 a2: aexp) (ans1 ans2: nat),
+  | E_APlus : forall s (a1 a2: aexp) (ans1 ans2: int64),
       aevalR s a1 ans1 ->
       aevalR s a2 ans2 ->
-      aevalR s (APlus a1 a2) (ans1 + ans2)
-  | E_AMinus: forall s (a1 a2: aexp) (ans1 ans2: nat),
+      aevalR s (APlus a1 a2) (Int64.add ans1 ans2)
+  | E_AMinus: forall s (a1 a2: aexp) (ans1 ans2: int64),
       aevalR s a1 ans1 ->
       aevalR s a2 ans2 ->
-      aevalR s (AMinus a1 a2) (ans1 - ans2)
-  | E_AMult : forall s (a1 a2: aexp) (ans1 ans2: nat),
+      aevalR s (AMinus a1 a2) (Int64.sub ans1 ans2)
+  | E_AMult : forall s (a1 a2: aexp) (ans1 ans2: int64),
       aevalR s a1 ans1 ->
       aevalR s a2 ans2 ->
-      aevalR s (AMult a1 a2) (ans1 * ans2).
+      aevalR s (AMult a1 a2) (Int64.mul ans1 ans2).
 Hint Constructors aevalR.
 
 Lemma aeval_iff_aevalR : forall s a ans, aeval s a = ans <-> aevalR s a ans.
@@ -101,8 +104,10 @@ Lemma compile_aexp_monotonic :
 Proof.
   intros g a.
   induction a; intros n1 m1 code1 v n2 m2 code2 Hcomp.  simpl in Hcomp.
-  - unfold_llvm Hcomp.
-    inversion Hcomp. repeat split; try omega. exists []. simpl; auto.
+  - simpl in Hcomp.
+    unfold_llvm Hcomp. simpl in Hcomp.
+    inversion Hcomp. repeat split; try omega.
+     exists [I (IId (lid_of_Z n1)) (INSTR_Op (SV (OP_IBinop (Add false false) i64 (val_of_int64 i) (val_of_int64 Integers.Int64.zero))))]. simpl; auto.
 
   - simpl in Hcomp.
     unfold_llvm Hcomp.
@@ -116,15 +121,13 @@ Proof.
 Qed.    
     
 
-
 Definition iid n (id:instr_id) : Prop := (IId (lid_of_Z n)) = id.
-
 Definition add_env_Z n dv (e:env) := add_env (lid_of_Z n) dv e.
 
 (* 
   The compiler emits code in "reverse" order, so when loaded into a CFG machine 
   
-*)
+
 Inductive code_at (CFG:mcfg) (f:function_id) (id_start:instr_id) : instr_id -> list elt -> Prop :=
 | code_at_nil : code_at CFG f id_start id_start []
 | code_at_uid :                         
@@ -133,7 +136,7 @@ Inductive code_at (CFG:mcfg) (f:function_id) (id_start:instr_id) : instr_id -> l
       (IHC: code_at CFG f id_start id code),
       code_at CFG f id_start id_next ((I id i)::code).
 Hint Constructors code_at.
-
+*)
 (*
 Inductive code_at (CFG:mcfg) (f:function_id) : list elt -> Prop := 
 | code_at_nil : code_at CFG f []
@@ -153,7 +156,7 @@ Inductive code_at (CFG:mcfg) (f:function_id) : list elt -> Prop :=
       code_at CFG f ((L bid)::code)
 .
 *)
-
+(*
 Lemma code_at_append_1 :
   forall (CFG:mcfg) (f:function_id) (code1 code2:list elt) k2 k0 (H:code_at CFG f k2 k0 (code1 ++ code2)),
     exists k1, code_at CFG f k1 k0 code1.
@@ -187,14 +190,23 @@ Proof.
   intros CFG f k1 k0 id i code H.
   inversion H. reflexivity.
 Qed.  
-
+*)
 (* These definitions should probably go in a library *)
-Definition dvalue_of_nat (n:nat) : value :=
-  DV (VALUE_Integer (Z.of_nat n)).
-Hint Unfold dvalue_of_nat.
 
-Definition Rv (v:value) (n:nat) : Prop := dvalue_of_nat n = v.
+(*
+Definition dvalue_of_nat (n:nat) : value :=
+  DVALUE_I64 (toi64 (Z.of_nat n)).
+Hint Unfold dvalue_of_nat.
+*)
+
+(* Related final values *)
+Definition  Rv (v:value) (i:int64) : Prop :=
+    v = DVALUE_I64 i.
 Hint Unfold Rv.
+
+(* Life Rv to error terms *)
+Inductive Rve : err value -> int64 -> Prop :=
+| Rve_inr : forall v i, Rv v i -> Rve (inr v) i.
 
 Lemma lookup_env_hd : forall id dv e, lookup_env (add_env id dv e) id = inr dv.
 Proof.
@@ -202,8 +214,6 @@ Proof.
   unfold add_env.
   rewrite Util.assoc_hd. reflexivity.
 Qed.  
-
-Require Import Program.
 
 Lemma lookup_env_tl : forall id1 v1 e id2 v2,
     id1 <> id2 -> lookup_env (add_env id1 v1 e) id2 = inr v2 <-> lookup_env e id2 = inr v2.
@@ -223,25 +233,59 @@ Proof.
     inversion H1.
 Qed.  
 
-Definition memory_invariant (g:ctxt) (e:env) n (m:memory) (st:Imp.state) : Prop :=
+Definition memory_invariant (g:ctxt) (e:env) (m:memory) (st:Imp.state) : Prop :=
   forall x v, g x = Some v ->
-         exists n', n' < n /\  (v = (local (lid_of_Z n')) /\
-                 exists a, (lookup_env e (lid_of_Z n') = inr (DVALUE_Addr a) /\
-                       Rv (nth_default undef m a) (st x))).
+         exists n, (v = (local (lid_of_Z n)) /\
+               exists a, (lookup_env e (lid_of_Z n) = inr (DVALUE_Addr a) /\
+                     Rv (nth_default undef m a) (st x))).
 
+Inductive env_lt (n:int) : env -> Prop :=
+| env_lt_nil : env_lt n []
+| env_lt_cons : forall e m dv, m < n -> env_lt n e -> env_lt n (add_env_Z m dv e)
+.                                                        
 
-Lemma memory_invariant_extension : forall g e n m st n' dv,
-  memory_invariant g e n m st -> n <= n' ->
-  memory_invariant g (add_env_Z n' dv e) n m st.
+Lemma env_lt_lookup_inv :
+  forall n n' e v
+    (Henv: env_lt n e)
+    (Hl: lookup_env e (lid_of_Z n') = inr v),
+    n' < n.
 Proof.
-  intros g e n m st n' dv Hm Hlt.
+  intros n n' e v Henv.
+  revert n' v.
+  unfold lookup_env. unfold trywith. unfold raise. 
+  induction Henv; intros n' v Hl.
+  - simpl in Hl. inversion Hl.
+  - unfold add_env_Z in Hl. unfold add_env in Hl.
+    unfold Util.assoc in Hl.
+    destruct (RawID.eq_dec (lid_of_Z n') (lid_of_Z m)).
+
+    Focus 2.
+    eapply IHHenv.
+    fold (@Util.assoc raw_id) in Hl.
+    destruct (Util.assoc RawID.eq_dec (lid_of_Z n') e).
+    exact Hl.
+    inversion Hl.
+
+    (* string_of n = string_of m -> n = m *)
+    unfold lid_of_Z in e0.
+Admitted.
+
+
+Lemma memory_invariant_extension : forall g e n mem st n' dv,
+    env_lt n e ->
+    n <= n' ->
+  memory_invariant g e mem st -> 
+  memory_invariant g (add_env_Z n' dv e) mem st.
+Proof.
+  intros g e n mem st n' dv Henv Hlt Hmem.
   unfold memory_invariant in *.
-  intros x v H.
-  destruct (Hm x v) as [n'' [Hlt' [Heq [a [HL HR]]]]]; auto.
-  exists n''. repeat split; auto.
-  exists a; split; auto.
-  unfold add_env_Z. eapply lookup_env_tl; eauto. apply lid_of_Z_inj.
-  unfold not. intros. subst. omega.
+  intros x v Hg.
+  apply Hmem in Hg. clear Hmem.
+  destruct Hg as [n0 [Hv [a [Ha Hrv]]]].
+  exists n0. split; auto.
+  exists a. eapply env_lt_lookup_inv with (n':=n0) in Henv.
+  split; auto. apply lookup_env_tl. apply lid_of_Z_inj.
+  unfold not. intros. subst. omega. auto. exact Ha.
 Qed.  
   
 (*
@@ -281,189 +325,151 @@ Proof.
 Qed.    
                                   
 
+Inductive straightline_code : list elt -> code -> Prop :=
+| slc_nil : straightline_code [] []
+| slc_cons : forall id i tl cd,
+    straightline_code tl cd ->
+    straightline_code ((I id i)::tl) ((id, i)::cd)
+.
+Hint Constructors straightline_code.
 
-
-(* LLVM A = ST (int * int * code) (err A) 
-   = (int * int * code) -> ((int * int * code) * err A)
-
-  e :: LLVM A
-  {P} e {x:Q} 
-  P int -> int -> code -> Prop 
-  Q int -> int -> code -> A -> Prop ->
-  forall n m code, 
-     P n m code  ->
-     exists n' m' code', 
-     e (n,m,code) = ((n',m',code'), inr res) ->
-     Q n' m' code' res
- *)
-(*
-Definition llvm_state := (int * int * list elt)%type.
-Definition LLVM_Pre := llvm_state -> Prop.
-Definition LLVM_Post (A:Type) := llvm_state -> llvm_state -> A -> Prop.
-
-Definition LLVM_INV {A} (P:LLVM_Pre) (lc:LLVM A) (Q:LLVM_Post A) :=
-  forall st,
-    P st ->
-    exists st' res,
-      (lc st = (st',inr res)) /\
-      (Q st st' res).
-
-Lemma llvm_ret_INV : forall {A} (P:LLVM_Pre) (Q:LLVM_Post A) v (Hpq: forall st, (P st -> Q st st v)),
-    LLVM_INV P (llvm_ret _ v) Q.
+Lemma straightline_code_app : forall x1 cd1 x2 cd2,
+    straightline_code x1 cd1 ->
+    straightline_code x2 cd2 ->
+    straightline_code (x1++x2) (cd1++cd2).
 Proof.
-  intros A P Q v Hpq.
-  unfold LLVM_INV.
-  intros st Hp.
-  exists st. exists v.
-  unfold llvm_ret; auto.
-Qed.
-
-Lemma llvm_bind_INV:
-  forall {A B} (P:LLVM_Pre) (Q:LLVM_Post A) (R:LLVM_Post B)
-    (e   : LLVM A)
-    (f   : A -> LLVM B)
-    (He  : LLVM_INV P e Q)
-    (Hf  : forall s v, LLVM_INV (fun s2 => Q s s2 v) (f v) R)
-    (Hqr : forall st st' st'' res res', Q st st' res -> R st' st'' res' -> R st st'' res')
-  ,
-    LLVM_INV P (llvm_bind _ _ e f) R.
-Proof.
-  intros A B P Q R e f He Hf Hqr. 
-  unfold llvm_bind.
-  unfold LLVM_INV in *.
-  intros st HP.
-  apply He in HP.
-  destruct HP as [st'[res[Heq HQ]]].
-  assert (Q st st' res) as HQ'. exact HQ.
-  apply Hf in HQ.
-  destruct HQ as [st''[res'[Heq' HR]]].
-  exists st''. exists res'. rewrite Heq.
-  split; auto. eapply Hqr.  apply HQ'. apply HR.
+  intros x1 cd1 x2 cd2 H.
+  revert x2 cd2.
+  induction H; intros x2 cd2 H0; auto. 
+  simpl. apply slc_cons. eapply IHstraightline_code. exact H0.
 Qed.  
 
-Definition start n := (IId (lid_of_Z n)).
+Definition slc_pc fn bid phis term cd :=
+  mk_pc fn (mk_block bid phis cd term).
 
-Definition CPre g e mem st : LLVM_Pre :=
-  fun (s:llvm_state) =>
-    memory_invariant g e mem st.
-
-Definition stepD_correct n code v ans :=
-  forall CFG fn e k mem,
-    code_at CFG fn (start n) code ->
-    exists pc' e' k' m' u,
-      step_star_invariant CFG (fun s m => s = (pc', e', k') /\ m' = m) (mk_pc fn (start n), e, k) mem
-      /\ eval_op e' v = inr u      
-      /\ Rv u ans.
-
-Definition CPost g e mem st ans (f : LLVM Ollvm_ast.value) : LLVM_Post Ollvm_ast.value :=
-  fun '((n,m,code):llvm_state) '((n',m',code'):llvm_state) (v:Ollvm_ast.value) =>
-    memory_invariant g e mem st /\
-    f (n,m,code) = (n',m',code', inr v) /\
-    exists code'', code' = code'' ++ code /\
-    stepD_correct n code'' v ans.
-
-Lemma compile_aexp_correct :
-  forall 
-    (a:aexp)
-    (st:Imp.state)
-    (ans:nat)
-    (Ha: aeval st a = ans)
-    (g:ctxt)
-    (f : LLVM Ollvm_ast.value)
-    (HComp: compile_aexp g a = f)
-    (mem:memory)
-    (e:env)
-  ,
-    LLVM_INV (CPre g e mem st) f (CPost g e mem st ans f).
+Lemma step_star_invariant_app2 :
+  forall CFG fn bid phis term,
+    let slc := slc_pc fn bid phis term in
+    forall R1 cd1 mem0 e0 k0
+      (HS1 : step_star_invariant CFG R1 ((slc cd1), e0, k0) mem0)
+      R2 cd2
+      (HR1 : forall st1 mem1, R1 st1 mem1 -> pc_of st1 = (slc []) /\
+                                          step_star_invariant CFG R2 ((slc cd2), env_of st1, stack_of st1) mem1),
+    step_star_invariant CFG R2 (slc (cd1++cd2), e0, k0) mem0.
 Proof.
-  intros a st ans Ha.
-  apply aeval_iff_aevalR in Ha.
-  induction Ha; intros g f HComp mem e.
-  - subst. simpl.
-    eapply llvm_ret_INV.
-    intros.
-    unfold CPre in H.
-    unfold CPost.
-    destruct st as [[n m] code].
-    split; eauto. unfold llvm_ret. split; eauto.
-    exists []. simpl. split; eauto.
-    unfold stepD_correct.
-    intros CFG fn e0 k mem0 H0.
-    exists (mk_pc fn (start n)). exists e0. exists k. exists mem0. exists (dvalue_of_nat ans).
-    simpl. split. eapply step_zero. split; eauto.
-    split. reflexivity. reflexivity.
-  - simpl in HComp.
-    unfold_llvm HComp.
-    unfold CPre.
-    unfold CPost.
-    unfold LLVM_INV.
-    intros [[n m] code] Hmem.
-    destruct (g id).
-    simpl in *.
-    subst. simpl.
-    exists (1 + n, m, I (IId (lid_of_Z n)) (INSTR_Load false i64 (i64ptr, v) None) :: code).
-    exists (local (lid_of_Z n)).
-    repeat split; auto.
-    exists [I (IId (lid_of_Z n)) (INSTR_Load false i64 (i64ptr, v) None)].
-    simpl. split; auto.
-    unfold stepD_correct.
-    intros CFG fn e0 k mem0 H.
-    exists (mk_pc fn (start n)).
-Abort.
-*)    
-(*    
-    subst. simpl.
-    eapply llvm_bind_INV.
-    Focus 2.
-    intros. 
-    eapply llvm_bind_INV.
-    Focus 2.
-    intros.
-    eapply llvm_ret_INV.
-    intros.
-    unfold CPost.
-    destruct st as [[n2 m2] code2].
-    split.
-*)    
-
+  intros CFG fn0 bid phis term slc R1 cd1.
+  induction cd1; intros mem0 e0 k0 HS1 R2 cd2 HR1.
+  - simpl in *. unfold slc in HS1. unfold slc_pc in HS1. 
+    + simpl.
+Admitted.        
   
+(*                                                   
+                      
+
+  step_star_invariant R1 (slc_pc fn bid phis 
+                         , e, k) mem 
+                      
+
+
+  step_star_invariant R (mk_pc fn
+                               {
+                                 blk_id = id;
+                                 blk_phis = phis;
+                                 blk_code = cd1 ++ cd2;
+                                 blk_term = term;
+                               }
+
+
+
+                         , e, k) mem 
+*)
+  
+Definition finish_pc (p:pc) : pc :=
+  let 'mk_pc f b := p in
+  mk_pc f
+  {| blk_id := blk_id b;
+    blk_phis := [];
+    blk_code := List.tl (blk_code b);
+    blk_term := blk_term b;
+  |}.
+
+
+Definition env_extends (e e':env) : Prop :=
+  forall op dv, eval_op e op = inr dv -> eval_op e' op  = inr dv.
+
+Lemma env_extends_lt :
+  forall e n n' dv
+    (Henv: env_lt n e)
+    (Hlt: n <= n'),
+    env_extends e (add_env_Z n' dv e).
+Proof.
+  intros e n n' dv Henv Hlt.
+  unfold env_extends.
+  intros op dv' Hev.
+  generalize dependent n.
+  revert n' dv.
+  destruct op as [op].
+  induction op; simpl in *; try inversion Hev; intros; subst; auto.
+  - destruct id; simpl in *; inversion H0.
+    unfold add_env_Z.
+    destruct (RawID.eq_dec (lid_of_Z n') id).
+    + subst. assert (n' < n). eapply env_lt_lookup_inv. apply Henv. apply H1.
+      rewrite H1.
+      apply lookup_env_tl.
+      apply lid_of_Z_inj. omega.
+      exact H1.
+    + rewrite H1.
+      apply lookup_env_tl; auto.
+  -
+    (* maybe cut down on cases from eval_expr to simplify for now. *)
+Admitted.    
+    
+    
+
 Lemma compile_aexp_correct :
   forall 
-    (a:aexp)
-    (st:Imp.state)
-    (ans:nat)
+    (a:aexp) (st:Imp.state) (ans:int64)
     (HAexp: aeval st a = ans)
 
     (g:ctxt)
-    n0
-    n m code
-    (Hlt:n0 <= n)
-    n' m' code'
+    (n m:int) (cd:list elt)
+    (n' m':int) (cd':list elt)
     (v : Ollvm_ast.value)
-    (Hcomp : compile_aexp g a (n,m,code) = ((n',m',code'),inr v))
+    (Hcomp : compile_aexp g a (n,m,cd) = ((n',m',cd'),inr v)),
 
+  exists cd_a c_a,
+    cd' = cd_a ++ cd
+    /\ straightline_code cd_a c_a
+    /\ forall
     (e:env)
+    (mem:memory) (n0:int)  (Hlt:n0 <= n)
+    (HM: memory_invariant g e mem st)
     (k:stack)
-    (mem:memory)
-    (HM: memory_invariant g e n0 mem st)
+    (CFG : mcfg)
+    (fn : function_id)
+    (bid: block_id)
+    phis term,
+      step_star_invariant
+        CFG
+        (fun s' mem' =>
+           let '(pc', e', k') := s' in
+           pc' = slc_pc fn bid phis term [] /\
+           memory_invariant g e' mem' st /\
+           Rve (eval_op e' v) ans /\
+           env_extends e e'
+        )
+        (slc_pc fn bid phis term (List.rev c_a), e, k) mem.
+      
+    exists (e':env) (u:dvalue), 
+      step_star_invariant
+        CFG
+        (fun s mem' => s = (slc_pc fn bid phis term [], e',k) /\ mem' = mem)
+        (slc_pc fn bid phis term (List.rev c_a), e, k) mem
 
-  ,
-  exists e' u,
-     memory_invariant g e' n0 mem st
-     /\
-     forall
-       (CFG : mcfg)
-       (fn : function_id)
-       (id_start:instr_id),
-       exists id_end,
-       forall (Hload: code_at CFG fn id_end id_start code'),
-    step_star_invariant
-      CFG (fun s mem' => s = (mk_pc fn id_end, e',k) /\ mem' = mem)
-      (mk_pc fn id_start, e, k) mem
-
-    /\ eval_op e' v = inr u      
-
-    /\ Rv u ans.
+       /\ memory_invariant g e' n0 mem st
+       /\ eval_op e' v = inr u      
+       /\ Rv u ans
+       /\ forall op w, eval_op e op = inr w -> eval_op e' op = inr w.
 Proof.
   intros a st ans HAexp.
   rewrite aeval_iff_aevalR in HAexp.
@@ -474,86 +480,119 @@ Proof.
   destruct H as [code0 HeqCode0].
   generalize dependent code0. generalize dependent n'. revert n m code v code' m'. 
 *)
-  induction HAexp; intros g n0 n m code Hlt n' m' code' v Hcomp e k mem HM.
-  Focus 1.
-  (* destruct (compile_aexp_monotonic _ _ _ _ _ _ _ _ _ Hcomp) as [Hlt1 [Hlt2 [code1 Heq]]]. *)
-    simpl in Hcomp. unfold_llvm Hcomp.
-    inversion Hcomp.
-    subst. exists e. exists (dvalue_of_nat ans).
-    split; auto.
-    intros CFG fn id_start. exists id_start.
-    split. eapply step_zero; auto. simpl. split. unfold dvalue_of_nat. reflexivity.
-    unfold Rv. reflexivity.
+  induction HAexp; intros g n m cd n' m' cd' v Hcomp.
+  - simpl in Hcomp. unfold_llvm Hcomp. simpl in Hcomp.
+    inversion Hcomp. clear Hcomp.
+    exists [I (IId (lid_of_Z n))
+         (INSTR_Op (SV (OP_IBinop (Add false false) i64 (val_of_int64 ans) (val_of_int64 Integers.Int64.zero))))].   exists [((IId (lid_of_Z n)),
+         (INSTR_Op (SV (OP_IBinop (Add false false) i64 (val_of_int64 ans) (val_of_int64 Integers.Int64.zero)))))].
+    repeat split; auto.
+    intros e mem n0 Hlt Hmem.
+    exists (add_env (lid_of_Z n) (DVALUE_I64 ans) e).
+    exists (DVALUE_I64 ans).
+    simpl.
+    repeat split; auto.
+    +  eapply step_tau. simpl. eauto.
+       eapply step_zero. split; auto.
+       repeat rewrite Int64.repr_signed. rewrite Int64.add_zero. reflexivity.
+    + eapply memory_invariant_extension; eauto.
+    + eapply lookup_env_hd.
 
-  Focus 2.
-    
+  - simpl in Hcomp. unfold_llvm Hcomp.
+    unfold trywith in Hcomp.
+    remember (g id) as X.
+    destruct X; simpl in Hcomp; try inversion Hcomp.
+    clear Hcomp.
+    exists [I (IId (lid_of_Z n)) (INSTR_Load false i64 (i64ptr, v0) None)].
+    exists [(IId (lid_of_Z n), (INSTR_Load false i64 (i64ptr, v0) None))].
+    simpl. repeat split; auto.
+    intros e mem n0 Hlt Hmem k CFG fn bid phis term.
+    destruct Hmem with (x:=id)(v:=v0) as [n1 [Hlt1 [Hv [a [Hlookup HRa]]]]]; auto.
+    exists (add_env (lid_of_Z n) (nth_default undef mem a) e).
+    exists (DVALUE_I64 (s id)). subst. 
+    repeat split; auto.
+      + subst. simpl. 
+        eapply step_eff. simpl.
+        rewrite Hlookup. simpl. eauto.
+        simpl. eauto.
+        simpl. eapply step_zero. simpl. split; auto.
+      + eapply memory_invariant_extension; eauto.
+      + rewrite lookup_env_hd.
+        inversion HRa as [H]. rewrite H.  reflexivity.
+        
   - simpl in Hcomp;
     unfold_llvm Hcomp;
-    specialize IHHAexp1 with (g:=g)(n0:=n0)(n:=n)(m:=m)(code:=code);
-    remember (compile_aexp g a1 (n, m, code)) as f;
-    destruct f as [[[n1 m1] code1] [err1|v1]];
-    try solve [inversion Hcomp];
-    lapply IHHAexp1; clear IHHAexp1; [intros IHHAexp1 | auto];
-(*    
-    apply eq_sym in Heqf.
-    assert (exists code11, code1 = code11 ++ code).
-    eapply compile_aexp_adds_code. apply Heqf.
-    destruct H as [code11 HeqCode11].
-*)
-    specialize IHHAexp1 with (n':=n1)(m':=m1)(code':=code1)(v:=v1);
-    lapply IHHAexp1; clear IHHAexp1; [intros IHHAexp1 | auto];
-    specialize IHHAexp1 with (e:=e)(k:=k)(mem:=mem);
-    lapply IHHAexp1; clear IHHAexp1; [intros IHHAexp1 | auto];
-    destruct IHHAexp1 as [e1 [u1 [HM1 H1]]];
+    specialize IHHAexp1 with (g:=g)(n:=n)(m:=m)(cd:=cd).
+    remember (compile_aexp g a1 (n, m, cd)) as f;
+    destruct f as [[[n1 m1] cd1] [err1|v1]];
+    try solve [inversion Hcomp].
+    specialize IHHAexp1 with (n':=n1)(m':=m1)(cd':=cd1)(v:=v1).
+    lapply IHHAexp1; clear IHHAexp1; [intros IHHAexp1 | auto].
+    destruct IHHAexp1 as [cd_a1 [c_a1 [Hcd_eq1 [HSlc1 IHHAexp1]]]].
 
     symmetry in Heqf;
     apply compile_aexp_monotonic in Heqf;
-    destruct Heqf as [ltn1 [ltm1 [code1' Heq_code1]]].
+    destruct Heqf as [ltn1 [ltm1 [cd1' Heq_cd1]]].
 
     
-    specialize IHHAexp2 with (g:=g)(n0:=n0)(n:=n1)(m:=m1)(code:=code1);
-    remember (compile_aexp g a2 (n1, m1, code1)) as f2;
-    destruct f2 as [[[n2 m2] code2] [err2|v2]];
-    try solve [inversion Hcomp];
-    lapply IHHAexp2; clear IHHAexp2; [intros IHHAexp2 | omega];
-    specialize IHHAexp2 with (n':=n2)(m':=m2)(code':=code2)(v:=v2);
-    lapply IHHAexp2; clear IHHAexp2; [intros IHHAexp2 | auto];
-    specialize IHHAexp2 with (e:=e1)(k:=k)(mem:=mem);
-    lapply IHHAexp2; clear IHHAexp2; [intros IHHAexp2 | auto];
-    destruct IHHAexp2 as [e2 [u2 [HM2 H2]]];
+    specialize IHHAexp2 with (g:=g)(n:=n1)(m:=m1)(cd:=cd1).
+    remember (compile_aexp g a2 (n1, m1, cd1)) as f2;
+    destruct f2 as [[[n2 m2] cd2] [err2|v2]];
+    try solve [inversion Hcomp].
+    specialize IHHAexp2 with (n':=n2)(m':=m2)(cd':=cd2)(v:=v2).
+    lapply IHHAexp2; clear IHHAexp2; [intros IHHAexp2 | auto].
+    destruct IHHAexp2 as [cd_a2 [c_a2 [Hcd_eq2 [HSlc2 IHHAexp2]]]].
 
     symmetry in Heqf2;
     apply compile_aexp_monotonic in Heqf2;
-    destruct Heqf2 as [ltn2 [ltm12[code2' Heq_code2]]].
+    destruct Heqf2 as [ltn2 [ltm2 [cd2' Heq_cd2]]].
 
 
     simpl in Hcomp.
     inversion Hcomp. clear Hcomp.
-    exists ((lid_of_Z n2, dvalue_of_nat (ans1 + ans2))::e2).
-    exists (dvalue_of_nat (ans1 + ans2)).
-    repeat split.
-    eapply memory_invariant_extension; [auto | omega].
 
-    intros.
-    specialize H1 with (CFG:=CFG)(fn:=fn)(id_start:=id_start).
-    destruct H1 as [id_end1 HA].
-    
-    Focus 3. 
     subst.
-    eapply step_star_invariant_app.
-    apply H1. 
-      assert ((I (IId (lid_of_Z n2)) (INSTR_Op (SV (OP_IBinop (Add false false) i64 v1 v2))) :: code2' ++ code1' ++ code) = ((I (IId (lid_of_Z n2)) (INSTR_Op (SV (OP_IBinop (Add false false) i64 v1 v2))) :: code2') ++ code1' ++ code)) by reflexivity.
-      rewrite H in Hload.
-      eapply code_at_append_2. apply Hload.
-      intros.  simpl in H. destruct H as [Hseq Hmeq].
-      subst.
-      eapply step_star_invariant_app.
-      eapply H2.
+    exists (I (IId (lid_of_Z n2)) (INSTR_Op (SV (OP_IBinop (Add false false) i64 v1 v2)))::cd2' ++ cd1').
+    exists (((IId (lid_of_Z n2)),(INSTR_Op (SV (OP_IBinop (Add false false) i64 v1 v2))))::c_a2 ++ c_a1).
+    simpl. repeat split.
+    + rewrite app_assoc. reflexivity.
+    + apply slc_cons. apply straightline_code_app; auto.
+      apply app_inv_tail in Hcd_eq2. rewrite Hcd_eq2. auto.
+      apply app_inv_tail in Hcd_eq1. rewrite Hcd_eq1. auto.
+    + intros e mem n0 Hlt0 Hmem k CFG fn bid phis term.
+      
+      specialize IHHAexp1 with (e:=e)(mem:=mem)(n0:=n0).
+      lapply IHHAexp1; clear IHHAexp1; [intros IHHAexp1 | auto].
+      lapply IHHAexp1; clear IHHAexp1; [intros IHHAexp1 | auto].
+      destruct IHHAexp1 with (k:=k)(CFG:=CFG)(fn:=fn)(bid:=bid)(phis:=phis)(term:=term)
+        as [e1 [u1 [HS1 [Hmem1 [Heval1 HRv1]]]]].
+      clear IHHAexp1.
 
-    
-    Focus 2.
-    + intros CFG fn Hload.
-      subst.
+      specialize IHHAexp2 with (e:=e1)(mem:=mem)(n0:=n0).
+      lapply IHHAexp2; clear IHHAexp2; [intros IHHAexp2 | auto].
+      lapply IHHAexp2; clear IHHAexp2; [intros IHHAexp2 | auto].
+      destruct IHHAexp2 with (k:=k)(CFG:=CFG)(fn:=fn)(bid:=bid)(phis:=phis)(term:=term)
+        as [e2 [u2 [HS2 [Hmem2 [Heval2 HRv2]]]]].
+      clear IHHAexp2.
+
+      exists (add_env (lid_of_Z n2) (DVALUE_I64 (Int64.add ans1 ans2)) e2). exists (DVALUE_I64 (Int64.add ans1 ans2)).
+      repeat split.
+      * rewrite rev_app_distr. eapply step_star_invariant_app2.
+        eapply step_star_invariant_app2.
+        apply HS1.
+        intros.
+        simpl in H. destruct H as [Hst1 Hmem1eq].
+        subst. simpl.
+        split. reflexivity.
+        apply HS2.
+        intros.
+        simpl in H. destruct H as [Hst2 Hmem2eq].
+        subst.
+        simpl. split. reflexivity.
+        eapply step_tau. simpl. rewrite Heval2. inversion HRv2. subst.
+        unfold slc_pc.
+      
+      
       
       
 
